\chapter{Synopsis of the weighted orbital integral $\Orb(\gamma, \phi, s)$ for $\gamma \in S_3(F)\rs$ and $\phi \in \HH(S_3(F))$}
\label{ch:orbital0}

This section defines the weighted orbital integral
and describes the parameters which we will use to express our answer.

\section{Initial definition of the weighted orbital integral for general $S_n(F)$}
Let $H = \GL_{n-1}(F)$.
Then $H$ has a natural embedding into $\GL_n(E)$ by
\[ h \mapsto \begin{pmatrix} h & 0 \\ 0 & 1 \end{pmatrix} \]
which endows it with an action $S_n(F)$.
Then our weighted orbital integral is defined as follows.
\begin{definition}
  [{\cite[Equation (3.2.3)]{ref:AFLspherical}}]
  \label{def:orbital0}
  For brevity let $\eta(h) \coloneqq \eta(\det h)$ for $h \in H$.
  For $\gamma \in S_n(F)$, $\phi \in \HH(S_n(F))$, and $s \in \CC$,
  we define the \emph{weighted orbital integral} by
  \[ \Orb(\gamma, \phi, s) \coloneqq
    \int_{h \in H} \phi(h\inv \gamma h) \eta(h)
    \left\lvert \det(h) \right\rvert_F^{-s} \odif h. \]
\end{definition}
\begin{definition}
  From now on we will abbreviate
  \[ \partial \Orb(\gamma, \phi)
    \coloneqq \left. \pdv{}{s} \right\rvert_{s=0} \Orb(\gamma, \phi, s). \]
\end{definition}


We remark that this weighted orbital integral is related to
an (unweighted) orbital integral on the unitary side
by the so-called relative fundamental lemma.
Specifically, for $g \in \U(\VV_n^+)$ and $f \in \HH(\U(\VV_n^+))$,
we define the (unweighted) orbital integral by
\[ \Orb^{\U(\VV_n^+)}(g, f) \coloneqq \int_{\U(\VV_n^+)} f(x^{-1}gx) \odif x. \]
Then the following result is true.
\begin{theorem}
  [Relative fundamental lemma; {\cite[Theorem 1.1]{ref:leslie}}]
  \label{thm:rel_fundamental_lemma}
  Let $\phi \in \HH(S_n(F))$ and $\gamma \in S_n(F)\rs$.
  \[ \omega(\gamma) \Orb(\phi, \gamma, 0)
    = \begin{cases}
      0 & \text{if }\gamma \in S_n(F)\rs^- \\
      \Orb^{\U(\VV_n^+)}(g, \BC^{\eta^{n-1}}_{S_n}(\phi)) & \text{if } \gamma \in S_n(F)\rs^+
    \end{cases}
  \]
  where the transfer factor $\omega$ is defined in \Cref{ch:geo}.
\end{theorem}

\section{Basis for the indicator functions in $\HH(S_3(F))$}
\label{ch:orbital0_hecke_basis}
From now on assume $n = 3$.
We have the symmetric space
\[ S_3(F) \coloneqq \left\{ g \in \GL_3(E) \mid g \bar{g} = \id_3 \right\}. \]
which has a left action under $\GL_3(E)$ by $g \cdot s \mapsto gs\bar{g}\inv$.

Then $S_3(F)$ admits the following decomposition, which we will use:
\begin{lemma}
  [Cartan decomposition of $S_3(F)$]
  For each integer $r \ge 0$ let
  \[ K'_{S,r} \coloneqq \GL_3(\OO_E) \cdot \begin{pmatrix} 0 & 0 & \varpi^r \\ 0 & 1 & 0 \\ \varpi^{-r} & 0 & 0 \end{pmatrix} \]
  denote the orbit of
  $\begin{pmatrix} 0 & 0 & \varpi^r \\ 0 & 1 & 0 \\ \varpi^{-r} & 0 & 0 \end{pmatrix}$
  under the left action of $\GL_3(\OO_E)$.
  Then we have a decomposition
  \[ S_3(F) = \coprod_{r \geq 0} K'_{S,r}. \]
\end{lemma}
\begin{proof}
  \todo{reference}
\end{proof}

The $r=0$ case will be given a special shorthand,
and can be expressed in a few equivalent ways:
\begin{align*}
  K'_S
  &\coloneqq K'_{S,0} \\
  &= \GL_3(\OO_E) \cdot \begin{pmatrix} & & 1 \\ & 1 \\ 1 \end{pmatrix} \\
  &= \GL_3(\OO_E) \cdot \id_3 = S_3(F) \cap \GL_3(\OO_E).
\end{align*}
One can equivalently define $K'_{S,r}$ to be the part of $S_3(F)$
for which the most negative valuation among the nine entries is $-r$.

For $r \geq 0$, define
\[ K'_{S, \le r} \coloneqq S_3(F) \cap \varpi^{-r} \GL_3(\OO_E). \]
We can re-parametrize the problem according to the following.
\begin{corollary}
  We have a decomposition
  \[ K'_{S, \le r} = K'_{S,0} \sqcup K'_{S,1} \sqcup \dots \sqcup K'_{S,r}. \]
\end{corollary}
Then an integral over each $K'_{S, \le r}$ lets us extract the integrals over $K'_{S,r}$.
\begin{corollary}
  For $r \ge 0$, the indicator functions $\mathbf{1}_{K'_{S, \le r}}$
  form a basis of $\HH(S_3(F))$.
\end{corollary}

Then, our goal is to compute for
$\partial \Orb(\gamma, \mathbf{1}_{K'_{S, \le r}})$
at $s=0$ for any $r > 0$ as well;
note that the $r = 0$ case is already done in \cite{ref:AFL}.

\section{Parametrization of $\gamma$}
Again, assume $n = 3$.
Further assume $\gamma \in S_3(F)\rs$ is regular semisimple.
We identify some parameters for the orbit of $\gamma$
that we can use for our explicit calculations.

\subsection{Rewriting the weighted orbital integral as a double integral over $E$
  via the group $H' \cong \GL_2(F)$}
Our weighted orbital integral is at present a quadruple integral over $F$,
owing to $H = \GL_{2}(F)$ being a four-dimensional $F$-vector space.

It will be more economical to work with the weighted orbital integral
as a double integral with two coefficients in $E$, in the following sense.
As in \cite[\S4.1]{ref:AFL} define
\[ H' \coloneqq
  \left\{ \begin{pmatrix} t_1 & t_2 \\ \bar t_2 & \bar t_1 \end{pmatrix}
    \mid t_1, t_2 \in E \right\}
\]
which is indeed a four-dimensional $F$-algebra.
As before $H' \hookrightarrow \U(\VV_n^+)$ according to the same embedding
$\GL_2(E) \hookrightarrow \GL_3(E)$
and so $H'$ also acts on $S_n(E)$ by conjugation.

As an $F$-algebra, we have an isomorphism (see \cite[\S4.1]{ref:AFL})
\begin{align*}
  \iota_2 \colon H = \GL_2(F)
  &\xrightarrow{\cong} H' \\
  \begin{pmatrix} a_{11} & a_{12} \\ a_{21} & a_{22} \end{pmatrix}
  &\mapsto \begin{pmatrix} t_1 & t_2 \\ \bar t_2 & \bar t_1 \end{pmatrix} \\
  t_1 &= \half\left( a_{11} + a_{22} + \frac{a_{12}}{\sqrt{\eps}} + a_{21} \sqrt{\eps} \right) \\
  t_2 &= \half\left( a_{11} - a_{22} + \frac{a_{12}}{\sqrt{\eps}} - a_{21} \sqrt{\eps} \right).
\end{align*}
Under this isomorphism, we have
\[ h \gamma h^{-1} = \iota_2(h) \gamma \overline{\iota_2(h)^{-1}}. \]

This allows us to rewrite the weighted orbital integral over $H'$ instead.
If we write $h' = \overline{\iota_2(h)^{-1}}$,
then the following integral formula is obtained.
\begin{proposition}
  [{\cite[\S4.2]{ref:AFL}}]
  \label{prop:orbital_over_H_prime}
  For brevity let $\eta(h') \coloneqq \eta(\det h')$ for $h' \in H'$.
  For $\gamma \in S_3(F)$, $\phi \in \HH(S_3(F))$, and $s \in \CC$,
  the weighted orbital integral can instead be written as
  \[ \Orb(\gamma, \phi, s) =
    \int_{h' \in H'} \phi(\bar{h'}\inv \gamma h') \eta(h')
    \left\lvert \det(h') \right\rvert_F^{s} \odif{h'} \]
  where
  \[ \odif{h'} = \kappa \cdot \frac{\odif t_1 \odif t_2}
    {\left\lvert t_1 \bar t_1 - t_2 \bar t_2 \right\rvert_F^2} \]
  for the constant
  \[ \kappa \coloneqq \frac{1}{(1-q\inv)(1-q^{-2})}. \]
\end{proposition}

\subsection{Identifying a representative in the $H'$-orbit}
Write $\gamma \overset{H'}{\sim} \gamma'$ to mean that $\gamma$ and $\gamma'$
are in the same $H'$-orbit.
Evidently the weighted orbital integral $\Orb(\gamma, \phi, s)$ in \Cref{prop:orbital_over_H_prime}
only depends on such an orbit.
So it makes sense to pick a canonical representative for the $H'$-orbit to compute
the weighted orbital integral in terms of.

Since we assumed $\gamma \in S_3(F)\rs$ is regular semisimple,
we can invoke \cite[Proposition 4.1]{ref:AFL}
to assume that $\gamma$ that under the orbit of $H'$ we have
\[ \gamma \overset{H'}{\sim}
  \begin{pmatrix}
    a & 0 & 0 \\
    b & - \bar d & 1 \\
    c & 1 - d \bar d & d
  \end{pmatrix}
  \in S_3(F)\rs; \quad \text{where $c = -a \bar b + b d$} \]
over all $a \in E^1$, $b \in E$, $d \in E$ for which $(1-d\bar d)^2 - c \bar c \neq 0$.
In other words, the representatives described here cover all the regular $H'$-orbits in $S_3(F)\rs$.

\subsection{Simplification due to the matching of non-quasi-split unitary group}
In this calculation, we restrict attention to the case where our regular $\gamma$
matches an element in the non-quasi-split unitary group $\U(\VV_n^-)\rs$
(rather than $\U(\VV_n^+)\rs$).
As we described in \Cref{prop:valuation_delta_matching_group},
this is controlled by the parity of the invariant
\[ v\left( (1-d\bar d)^2 - c \bar c\right) \]
being odd.
Hence, we only have to consider this case:
\begin{assume}
  \label{assume:u_odd}
  We will assume that
  \[ v\left( (1-d\bar d)^2 - c \bar c\right) \equiv 1 \pmod 2. \]
\end{assume}
This is the same assumption made in \cite[Equation (4.3)]{ref:AFL}.

To summarize everything we've said.
\begin{lemma}
  \label{lem:S3_abcd}
  Let $\gamma \in S_3(F)\rs^-$.
  Then there exists $a \in E^1$, $b \in E$, $d \in E$ such that
  \[ \gamma \overset{H'}{\sim}
    \begin{pmatrix}
      a & 0 & 0 \\
      b & - \bar d & 1 \\
      c & 1 - d \bar d & d
    \end{pmatrix}
    \in S_3(F)\rs; \quad \text{where $c = -a \bar b + b d$}. \]
  Moreover, $v\left( (1-d \bar d)^2 - c \bar c \right)$ is odd.
\end{lemma}

We will mostly be interested in the case where $v(b) = v(d) = 0$.
In fact, few other cases even occur at all given \Cref{assume:u_odd};
we will see momentarily that either $v(b) = v(d) < 0$,
or one of $\{v(b), v(d)\}$ is zero and the other is nonnegative.

\section{Parameters used in the calculation of the weighted orbital integral}
\label{sec:param_orbital0}

We now evaluate the orbital integral in terms of
\[ a \in E^1, \qquad b, d \in E, \qquad r \ge 0. \]
To simplify the notation in what follows,
it will be convenient to define several quantities that reappear frequently.
From \Cref{assume:u_odd}, we may define
\begin{equation}
  \delta \coloneqq v(1-d \bar d) = v(c) \neq -\infty.
  \label{eq:delta}
\end{equation}
Following \cite[Equation (4.3)]{ref:AFL} we will also define
\begin{equation}
  u \coloneqq \frac{\bar c}{1-d \bar d} \in \OO_E^\times
  \label{eq:u}
\end{equation}
so that $\nu(1-u \bar u) \equiv 1 \pmod 2$ and
\begin{equation}
  b = -au - \bar{d} \bar{u}.
  \label{eq:b}
\end{equation}
Note that this gives us the following repeatedly used identity
\begin{equation}
  b^2-4a\bar d = (au-\bar d \bar u)^2 - 4a\bar d(1-u\bar u).
  \label{eq:dos}
\end{equation}
Finally, define
\begin{equation}
  \ell \coloneqq v(b^2 - 4 a \ol d).
  \label{eq:ell}
\end{equation}
We will also define one additional parameter useful when $\ell$ is even
(but as we will see, redundant for odd $\ell$):
\begin{equation}
  \lambda \coloneqq v(1-u \bar u) \equiv 1 \pmod 2.
  \label{eq:lambda}
\end{equation}

Just as many pairs $(v(b), v(d))$ do not occur (given \Cref{assume:u_odd})
and $v(b) = v(d) = 0$ is the main case of interest,
the parameters $(\delta, \ell, \lambda)$ satisfy some additional relations.
We will now describe them.

\begin{lemma}
  \label{lem:parameter_constraints}
  Let $a$, $b$, $c$, $d$ be as in \Cref{lem:S3_abcd},
  and let $\delta$, $\ell$, and $\lambda$ be as defined in
  \eqref{eq:delta}, \eqref{eq:ell}, \eqref{eq:lambda}.
  Then exactly one of the following situations is true:
  \begin{itemize}
    \ii $v(b) = v(d) = 0$, $\ell \ge 1$ is odd, $\ell < 2 \delta$, and $\lambda = \ell$.
    \ii $v(b) = v(d) = 0$, $\ell \ge 0$ is even, $\ell \le 2 \delta$, and $\lambda > \ell$ is odd.
    \ii $v(b) = 0$, $v(d) > 0$, $\ell = \delta = 0$, and $\lambda > 0$ is odd.
    \ii $v(b) > 0$, $v(d) = 0$, $\ell = 0$, $\delta \ge 0$, and $\lambda > 0$ is odd.
    \ii $v(b) = v(d) < 0$, $\ell = \delta = 2v(d) < 0$, and $\lambda > 0$ is odd.
  \end{itemize}
  See \Cref{tab:parameter_constraints}.
  Moreover, whenever $\ell$ is even,
  the quantity $b^2 - 4 a \bar d$ is a square of some element in $E$.
\end{lemma}

\begin{table}[ht]
  \centering
  \begin{tabular}{cccc}
    \toprule
    & $v(b) = 0$ & $v(b) > 0$ & $v(b) < 0$ \\
    \midrule
    $v(d) = 0$ & $0 \le \ell \le 2 \delta$ & $\ell = 0$, $\delta \ge 0$ & never \\
    $v(d) > 0$ & $\ell = \delta = 0$ & never & never \\
    $v(d) < 0$ & never & never & $v(b) = v(d) = \frac{\ell}{2} = \frac{\delta}{2} < 0$ \\
    \bottomrule
  \end{tabular}
  \caption{A table showing the five cases in \Cref{lem:parameter_constraints}.}
  \label{tab:parameter_constraints}
\end{table}

Before proving the lemma in full we first prove the following lemmas.
\begin{lemma}
  \label{lem:au_minus_du}
  Assume $v(d) \ge 0$.
  For odd $\ell$, we have
  \[ 2 v(au - \bar d \bar u) > \ell = \lambda \]
  while for even $\ell$ we instead have
  \[ 2 v(au - \bar d \bar u) = \ell < \lambda. \]
\end{lemma}
\begin{proof}
  If $v(d) = 0$, this follows from \eqref{eq:dos} directly,
  since $v\left( (au - \bar d \bar u)^2 \right)$ is even, and hence
  can never equal $v(4a \bar d (1- u \bar u)) = \lambda \equiv 1 \pmod 2$.

  Meanwhile, if $v(d) > 0$, then from \eqref{eq:b}
  it follows $v(b) = 0$, and hence $\ell = 0$.
  And $v(au - \bar d \bar u) = 0$ in this case as well.
  Since $\lambda$ is a positive odd integer, the lemma is proved.
\end{proof}

\begin{lemma}
  If $v(b) = v(d) = 0$ and $\ell \ge 0$, then $\ell \le 2 \delta$.
  \label{lem:ell_le_2_delta}
\end{lemma}
\begin{proof}
  If $\ell = 0$ there is nothing to prove so assume $\ell > 0$.
  Let us write
  \begin{equation}
    \OO_E^\times \ni \frac{a d u}{\bar u} = x + y \sqrt{\eps} \qquad x,y \in F
    \label{eq:ell_delta_adu_xy}
  \end{equation}
  which has norm
  \begin{equation}
    \OO_F^\times \ni x^2+y^2\eps
    = \frac{a d u}{\bar u} \cdot \frac{\bar a \bar d \bar u}{u} = d \bar d.
    \label{eq:ell_delta_adu_norm}
  \end{equation}

  Now, according to \Cref{lem:au_minus_du} we have that
  \[ 0 < \ell \le 2v(au - \bar d \bar u)
    = 2v\left( \frac{a d u}{\bar u} - d \bar d \right)
    = 2v\left(  (x - d \bar d) + y \sqrt{\eps}. \right) \]
  and since $d \bar d \in F$, it follows that
  \begin{align}
    v\left( x - d \bar d \right) &> \frac{\ell}{2} \label{eq:ell_delta_x_minus_d_bar_d} \\
    v(y) &> \frac{\ell}{2}. \label{eq:ell_delta_y}
  \end{align}
  In particular, \eqref{eq:ell_delta_y} implies $v(y) > 0$ which has two consequences:
  \begin{itemize}
    \ii From \eqref{eq:ell_delta_adu_xy} we get $v(x) = 0$.
    \ii From $v(y^2) > 0$ and \eqref{eq:ell_delta_adu_norm}
    we conclude \[ v(x^2 - d \bar d) = v(y^2) > \ell. \]
  \end{itemize}
  Putting \eqref{eq:ell_delta_x_minus_d_bar_d} together with the previous two bullets,
  \[ \frac{\ell}{2} \le v\left( x^2 - d \bar d - x(x - d \bar d) \right)
    = v(x) + v(1-d \bar d) = 0 + \delta \]
  and this proves $\ell \le 2\delta$.
\end{proof}

Now we can prove \Cref{lem:parameter_constraints}.
\begin{proof}[Proof of \Cref{lem:parameter_constraints}]
  It's clear the five bullets above are disjoint.
  \begin{itemize}
  \ii First assume $\ell$ is odd.
  We assert in this case we have $v(b) = v(d) = 0$.
  Indeed if $v(d) \neq 0$, then $b = -au-\bar d\bar u$ is a unit,
  and hence so is $b^2 - 4 a \bar d$, causing $\ell = 0$, contradiction.
  And if $d$ is a unit, $\ell \neq 0$ means $v(b) = 0$ too.
  In particular, $\ell > 0$.
  The rest of the claims follow by \Cref{lem:au_minus_du} and \Cref{lem:ell_le_2_delta}.
  \end{itemize}
  For the rest of the proof we only consider even $\ell$.
  Because $b = -au - \bar d \bar u$, it cannot be the case that $v(b) > 0$ and $v(d) > 0$;
  moreover if either $v(b) < 0$ or $v(d) < 0$,
  then in fact $v(b) = v(d)$.
  We consider each of the four possibilities.
  \begin{itemize}
  \ii Suppose and $v(b) = v(d) = 0$.
  Then \Cref{lem:au_minus_du} and \Cref{lem:ell_le_2_delta} imply the results.

  \ii If $v(b) = 0$ and $v(d) > 0$, then $b^2 - 4a \bar d$ is a unit
  and $1 - d \bar d$ are both units, ergo $\ell = \delta = 0$.

  \ii If $v(b) > 0$ and $v(d) = 0$ then $b^2 - 4 a \bar d$ is a unit,
  and there is nothing left to prove.

  \ii Finally suppose $v(b) = v(d) < 0$.
  Then $v(b^2) < v(4 a \bar d) < 0$, so indeed $\ell = 2 v(d) < 0$.
  And $v(1 - d \bar d) = 2v(d) < 0$ as well.
  \end{itemize}
  We now verify the last assertion that $b^2 - 4 a \bar d$
  is a square whenever $\ell$ is even.
  The proof in all cases uses \eqref{eq:dos} to show $b^2 - 4 a \bar d$
  is equal to $\varpi^\ell$ times a quadratic residue in $\OO_E^\times$.
  Indeed we need only verify that $v(4a \bar d(1 - u \bar u)) = v(d) + \lambda$
  has larger valuation than $v\left( (a u - \bar d \bar u)^2 \right) = \ell$.
  In the case $v(b) = 0$ this follows from $\lambda > \ell$.
  Whereas if $v(d) > 0$ we have $\ell = 0$
  and if $v(b) = v(d) < 0$ then $\ell = -2v(d)$;
  so in all these cases the claim is obvious too. \qedhere
\end{proof}

In the case where $\ell$ is odd (and hence $\ell \ge 1$ and $v(b) = v(d) = 0$),
we get \eqref{eq:dos} implying $\lambda = \ell$
and thus $\lambda$ will never be used --- the weighted orbital will be computed
as a function of $\ell$ and $\delta$ (and $r$).

However for even $\ell$ these numbers are never equal and our weighted orbital
integral will be stated in terms of $\ell$, $\delta$, and $\lambda$ (and $r$).
We just saw that in these situations $b^2 - 4 a \bar d$ is a square;
moving forward, we need to fix the choice of the square root $\tau$.
We do so as follows.
\begin{definition}
  [Fixing the choice of $\tau$]
  Assuming $\ell$ is even, using \eqref{eq:dos} in the form
  \[ (au-\bar d \bar u)^2 - \tau^2 = 4a\bar d(1- u\bar u) \]
  we agree now to fix the choice of the square root of $\tau$ such that
  \begin{equation}
    \begin{aligned}
      v(au-\bar d \bar u + \tau) &= \lambda + v(d) - \half \ell > 0, \\
      v(au-\bar d \bar u - \tau) &= \half \ell.
    \end{aligned}
    \label{eq:tau_choice}
  \end{equation}
\end{definition}
Here $\lambda + v(d) - \half \ell > 0$ is obvious when $v(d) \ge 0$
(since $\lambda = \ell > 0$ for odd $\ell$ and otherwise $\lambda > \ell$),
and for $v(d) < 0$ we have $v(d) = \half \ell$ anyway.

\begin{lemma}
  With this choice of $\tau$, we have
  \begin{equation}
    \begin{aligned}
      v\left( 4 - \Norm(b+\tau) \right) &= \lambda + \delta - \ell \\
      v\left( 4 - \Norm(b-\tau) \right) &= \delta.
    \end{aligned}
    \label{eq:four_norm_choice}
  \end{equation}
\end{lemma}
\begin{proof}
  We consider several cases.
  \begin{itemize}
  \ii If $v(b) = v(d) = 0$ then from \eqref{eq:dos} we have
  \[ \ell = 2v(\tau) = 2v(au - \bar d \bar u) < \lambda \]
  and thus \cite[Lemma 4.7]{ref:AFL} applies to give \eqref{eq:four_norm_choice}, verabtim.

  \ii Now suppose $v(d) > 0$ but still $v(b) = v(\tau) = 0$.
  We begin with the observation that
  \begin{equation}
    4 a \bar d = b^2 - \tau^2 = (b + \tau)(b - \tau)
    \label{eq:tau_which_which}
  \end{equation}
  and so $\{v(b+\tau), v(b-\tau)\} = \{0, v(d)\}$.
  We need to determine which is which.
  However, note that we may write
  \[ au - \bar d \bar u - \tau = -(b + \tau) - 2 \bar d \bar u. \]
  Since $v(au - \bar d \bar u - \tau) = 0$ and $v(d) > 0$,
  it follows we must have $v(b+\tau) = 0$.
  And thus $v(b-\tau) = v(d)$.
  Hence $v(4 - \Norm(b-\tau)) = 0 = \delta$,
  and we have obtained the bottom equation of \eqref{eq:four_norm_choice}.

  It remains to show that $v(4-\Norm(b+\tau)) = \lambda$ to complete the proof.
  We quote \cite[Lemma 4.6]{ref:AFL} which states more generally that
  \begin{align*}
    2\delta + \lambda
    &= v(4-\Norm(b+\tau)) + v(4-\Norm(b-\tau)) \\
    &\qquad+ v(16 + 16 d \bar d - 8 b \bar b + 8 \tau \bar\tau).
  \end{align*}
  In our case $\delta = 0$, $v(4-\Norm(b-\tau)) = 0$.
  Moreover since $v(\tau - b) > 0$ we get $v(\tau\bar\tau - b \bar b) > 0$.
  (Indeed, if $\tau = x_\tau + \eps y_\tau$ and $b = x_b + \eps y_b$,
  then $\tau\bar\tau - b \bar b = (x_\tau^2 - x_b^2 + \eps(y_\tau^2 - y_b^2))
  + \eps(x_\tau y_\tau - y_\tau y_b)$.
  Since $x_\tau \equiv x_b \pmod{\varpi}$ and $y_\tau \equiv y_b \pmod{\varpi}$,
  the conclusion is immediate.)
  Hence the final term on the right-hand side is $0$ too.

  \ii Consider $v(b) > 0$.
  As mentioned on \cite[p.\ 242]{ref:AFL}, the identity \eqref{eq:four_norm_choice}
  is still true in this situation too.

  \ii Finally assume $v(\tau) = v(b) = v(d) < 0$.
  Again from \eqref{eq:tau_which_which}
  we know $\{v(b+\tau), v(b-\tau)\} = \{0, v(d)\}$ and need to determine which is which.
  This time we write
  \[ au - \bar d \bar u + \tau = -(b - \tau) - 2 \bar d \bar u. \]
  Since $v(au - \bar d \bar u + \tau) = \lambda > 0$,
  but $v(2 \bar d \bar u) = v(d) < 0$,
  it follows we must have $v(b-\tau) < 0$,
  so in fact $v(b-\tau) = v(d)$ and $v(b+\tau) = 0$.
  So, in this case, we get $v(4 - \Norm(b-\tau)) = 2v(b) = \delta$,
  which is the bottom equation of \eqref{eq:four_norm_choice}.

  Then it remains to show that $v(4-\Norm(b+\tau)) = \lambda$,
  which is done in the same way as $v(d) > 0$ earlier.
  \qedhere
  \end{itemize}
\end{proof}
